yalla/ill_smp.v
@@ -1,6 +1,3 @@
-(* ill example file for yalla library *)
-
-
 (** * Example of a concrete use of the yalla library: ILL *)
 
 From Coq Require Import CMorphisms.
@@ -16,19 +13,14 @@ Set Implicit Arguments.
 
 Section Atoms.
 
-Context { preiatom : DecType }.
+Context {preiatom : DecType}.
 
 (** ** 1. define formulas *)
 Inductive iformula :=
-| ivar  : @iformulas.iatom preiatom -> iformula
-| ione  : iformula
-| itens : iformula -> iformula -> iformula
-| ilmap : iformula -> iformula -> iformula
-| itop  : iformula
-| iwith : iformula -> iformula -> iformula
-| izero : iformula
-| iplus : iformula -> iformula -> iformula
-| ioc   : iformula -> iformula.
+| ivar (_ : @iformulas.iatom preiatom)
+| ione | itens (_ _ : iformula) | ilmap (_ _ : iformula)
+| itop | iwith (_ _ : iformula) | izero | iplus (_ _ : iformula)
+| ioc (_ : iformula).
 
 
 (** ** 2. define embedding into [formulas.formula] *)
@@ -48,58 +40,51 @@ end.
 
 Lemma ill2ill_inj : injective ill2ill.
 Proof.
-intros A.
-induction A ; intros B Heq ;
-  destruct B ; inversion Heq ;
-  try apply IHA in H0 ;
-  try apply IHA1 in H0 ;
-  try apply IHA2 in H1 ; subst ;
-  reflexivity.
+intros A. induction A; intros B Heq; destruct B; inversion Heq;
+  try apply IHA in H0; try apply IHA1 in H0; try apply IHA2 in H1; subst; reflexivity.
 Qed.
 
-Lemma ill2ill_map_ioc l :
-  map ill2ill (map ioc l) = map iformulas.ioc (map ill2ill l).
+Lemma ill2ill_map_ioc l : map ill2ill (map ioc l) = map iformulas.ioc (map ill2ill l).
 Proof. induction l as [|a l IHl]; [ | cbn; rewrite IHl ]; reflexivity. Qed.
 
 Lemma ill2ill_map_ioc_inv l1 l2 :
-  map iformulas.ioc l1 = map ill2ill l2 ->
-    { l2' | l2 = map ioc l2' /\ l1 = map ill2ill l2' }.
+  map iformulas.ioc l1 = map ill2ill l2 -> { l2' | l2 = map ioc l2' & l1 = map ill2ill l2' }.
 Proof.
 induction l1 in l2 |- *; intros Heq; destruct l2; inversion Heq.
-- exists nil; split; reflexivity.
+- exists nil; reflexivity.
 - apply IHl1 in H1.
   destruct i; inversion H0; subst.
-  destruct H1 as (l2' & Heq1 & H1); subst.
-  exists (i :: l2'); split; reflexivity.
+  destruct H1 as [l2' -> ->].
+  exists (i :: l2'); reflexivity.
 Qed.
 
 
 (** ** 3. define proofs *)
 
 Inductive ill : list iformula -> iformula -> Type :=
-| ax_ir : forall X, ill (ivar X :: nil) (ivar X)
-| ex_ir : forall l1 l2 A, ill l1 A -> Permutation_Type l1 l2 -> ill l2 A
+| ax_ir X : ill (ivar X :: nil) (ivar X)
+| ex_ir l1 l2 A : ill l1 A -> Permutation_Type l1 l2 -> ill l2 A
 | one_irr : ill nil ione
-| one_ilr : forall l A, ill l A -> ill (ione :: l) A
-| tens_irr : forall A B l1 l2, ill l1 A -> ill l2 B -> ill (l1 ++ l2) (itens A B)
-| tens_ilr : forall A B l C, ill (A :: B :: l) C -> ill (itens A B :: l) C
-| lmap_irr : forall A B l, ill (A :: l) B -> ill l (ilmap A B)
-| lmap_ilr : forall A B l1 l2 C, ill l1 A -> ill (B :: l2) C -> ill (ilmap A B :: l1 ++ l2) C
-| top_irr : forall l, ill l itop
-| with_irr : forall A B l, ill l A -> ill l B -> ill l (iwith A B)
-| with_ilr1 : forall A B l C, ill (A :: l) C -> ill (iwith A B :: l) C
-| with_ilr2 : forall A B l C, ill (A :: l) C -> ill (iwith B A :: l) C
-| zero_ilr : forall l C, ill (izero :: l) C
-| plus_irr1 : forall A B l, ill l A -> ill l (iplus A B)
-| plus_irr2 : forall A B l, ill l A -> ill l (iplus B A)
-| plus_ilr : forall A B l C, ill (A :: l) C -> ill (B :: l) C -> ill (iplus A B :: l) C
-| oc_irr : forall A l, ill (List.map ioc l) A -> ill (List.map ioc l) (ioc A)
-| de_ilr : forall A l C, ill (A :: l) C -> ill (ioc A :: l) C
-| wk_ilr : forall A l C, ill l C -> ill (ioc A :: l) C
-| co_ilr : forall A l C, ill (ioc A :: ioc A :: l) C -> ill (ioc A :: l) C.
+| one_ilr l A : ill l A -> ill (ione :: l) A
+| tens_irr A B l1 l2 : ill l1 A -> ill l2 B -> ill (l1 ++ l2) (itens A B)
+| tens_ilr A B l C : ill (A :: B :: l) C -> ill (itens A B :: l) C
+| lmap_irr A B l : ill (A :: l) B -> ill l (ilmap A B)
+| lmap_ilr A B l1 l2 C : ill l1 A -> ill (B :: l2) C -> ill (ilmap A B :: l1 ++ l2) C
+| top_irr l : ill l itop
+| with_irr A B l : ill l A -> ill l B -> ill l (iwith A B)
+| with_ilr1 A B l C : ill (A :: l) C -> ill (iwith A B :: l) C
+| with_ilr2 A B l C : ill (A :: l) C -> ill (iwith B A :: l) C
+| zero_ilr l C : ill (izero :: l) C
+| plus_irr1 A B l : ill l A -> ill l (iplus A B)
+| plus_irr2 A B l : ill l A -> ill l (iplus B A)
+| plus_ilr A B l C : ill (A :: l) C -> ill (B :: l) C -> ill (iplus A B :: l) C
+| oc_irr A l : ill (List.map ioc l) A -> ill (List.map ioc l) (ioc A)
+| de_ilr A l C : ill (A :: l) C -> ill (ioc A :: l) C
+| wk_ilr A l C : ill l C -> ill (ioc A :: l) C
+| co_ilr A l C : ill (ioc A :: ioc A :: l) C -> ill (ioc A :: l) C.
 
 Instance ill_perm C : Proper ((@Permutation_Type _) ==> arrow) (fun l => ill l C).
-Proof. intros l1 l2 HP pi; eapply ex_ir; eassumption. Qed.
+Proof. intros l1 l2 HP pi. eapply ex_ir; eassumption. Qed.
 
 (** ** 4. characterize corresponding [ill] fragment *)
 
@@ -111,139 +96,130 @@ Definition ill_ll := ill_def.ill ipfrag_ill.
 
 Lemma ill2illfrag l A : ill l A -> ill_ll (map ill2ill l) (ill2ill A).
 Proof.
-intros pi; induction pi; rewrite <- (app_nil_l _); try (now constructor); rewrite ? map_app.
+intros pi. induction pi; rewrite <- (app_nil_l _); try (now constructor); rewrite ? map_app.
 - eapply ill_def.ex_ir; [ eassumption | ].
-  apply Permutation_Type_map; assumption.
-- rewrite app_nil_l; constructor; assumption.
+  apply Permutation_Type_map. assumption.
+- rewrite app_nil_l. constructor; assumption.
 - eapply ill_def.ex_ir.
-  + cbn in IHpi2; rewrite <- (app_nil_l _) in IHpi2.
-    apply (ill_def.lmap_ilr _ _ _ _ _ _ IHpi1 IHpi2).
-  + cbn; symmetry; apply Permutation_Type_cons_app; rewrite map_app; reflexivity.
-- cbn; rewrite ill2ill_map_ioc.
-  apply ill_def.oc_irr.
-  rewrite <- ill2ill_map_ioc; assumption.
+  + cbn in IHpi2. rewrite <- (app_nil_l _) in IHpi2. exact (ill_def.lmap_ilr _ _ _ _ _ _ IHpi1 IHpi2).
+  + cbn. symmetry. apply Permutation_Type_cons_app. rewrite map_app. reflexivity.
+- cbn. rewrite ill2ill_map_ioc. apply ill_def.oc_irr.
+  rewrite <- ill2ill_map_ioc. assumption.
 Qed.
 
 Lemma illfrag2ill l A : ill_ll (map ill2ill l) (ill2ill A) -> ill l A.
 Proof.
 intros pi.
-remember (map ill2ill l) as l0; remember (ill2ill A) as A0.
+remember (map ill2ill l) as l0 eqn:Heql0. remember (ill2ill A) as A0 eqn:HeqA0.
 revert l Heql0 A HeqA0; induction pi; intros l' Heql0 A' HeqA0; subst;
   try (now inversion f);
   try (now destruct A'; inversion HeqA0; subst;
          try (symmetry in Heql0; decomp_map_inf Heql0; subst); constructor;
-         try (now apply IHpi);
-         try (now apply IHpi1);
-         try (now apply IHpi2)).
+         try (now apply IHpi); try (now apply IHpi1); try (now apply IHpi2)).
 - destruct A'; inversion HeqA0.
   destruct l'; inversion Heql0; destruct l'; inversion Heql0.
   destruct i0; inversion H3; subst.
   apply ax_ir.
-- cbn in p.
-  apply Permutation_Type_map_inv in p as [l'' Heq HP%Permutation_Type_sym].
+- cbn in p. apply Permutation_Type_map_inv in p as [l'' Heq HP%Permutation_Type_sym].
   eapply ex_ir; [ | eassumption ].
   apply IHpi; [ assumption | reflexivity ].
-- symmetry in Heql0; decomp_map_inf Heql0; subst.
-  cbn in Heql0; symmetry in Heql0; apply ill2ill_map_ioc_inv in Heql0;
-    destruct Heql0 as (l & -> & ->).
+- symmetry in Heql0. decomp_map_inf Heql0. subst.
+  cbn in Heql0. symmetry in Heql0. apply ill2ill_map_ioc_inv in Heql0 as [l -> ->].
   apply Permutation_Type_map_inv in p as [l' -> HP%Permutation_Type_sym].
-  eapply ex_ir;
-    [ apply IHpi; [ | reflexivity];
-      rewrite <- ill2ill_map_ioc, <- ? map_app; reflexivity | ].
-  apply Permutation_Type_app_head, Permutation_Type_app_tail, Permutation_Type_map; assumption.
+  eapply ex_ir; [ apply IHpi; [ | reflexivity];
+                  rewrite <- ill2ill_map_ioc, <- ? map_app; reflexivity | ].
+  apply Permutation_Type_app_head, Permutation_Type_app_tail, Permutation_Type_map. assumption.
 - destruct A'; inversion HeqA0.
   destruct l'; inversion Heql0.
   apply one_irr.
-- symmetry in Heql0; decomp_map_inf Heql0; subst.
+- symmetry in Heql0. decomp_map_inf Heql0. subst.
   destruct x; inversion Heql0.
   eapply ex_ir.
   + apply one_ilr.
-    apply IHpi; [ rewrite <- ? map_app | ]; reflexivity.
+    apply IHpi; [ rewrite <- ! map_app | ]; reflexivity.
   + apply Permutation_Type_middle.
-- symmetry in Heql0; decomp_map_inf Heql0; subst.
+- symmetry in Heql0. decomp_map_inf Heql0. subst.
   destruct x; inversion Heql0; subst.
   eapply ex_ir.
   + apply tens_ilr.
     eapply (@ex_ir _ (x1 :: x2 :: l0 ++ l4)).
     * apply (IHpi (l0 ++ x1 :: x2 :: l4)); [ cbn; rewrite map_app | ]; reflexivity.
-    * symmetry; apply Permutation_Type_cons_app, Permutation_Type_middle.
+    * symmetry. apply Permutation_Type_cons_app, Permutation_Type_middle.
   + apply Permutation_Type_middle.
-- symmetry in Heql0; decomp_map_inf Heql0; subst.
-  destruct x ; inversion Heql0.
-- symmetry in Heql0; decomp_map_inf Heql0; subst.
+- symmetry in Heql0. decomp_map_inf Heql0. subst.
+  destruct x; inversion Heql0.
+- symmetry in Heql0. decomp_map_inf Heql0. subst.
   destruct x; inversion Heql2.
-- symmetry in Heql0; decomp_map_inf Heql0; subst.
+- symmetry in Heql0. decomp_map_inf Heql0. subst.
   destruct x; inversion Heql3; subst.
   eapply ex_ir.
   + apply lmap_ilr.
     * apply IHpi1; reflexivity.
     * eapply (@ex_ir (l3 ++ x2 :: l7) (x2 :: l3 ++ l7)).
       -- apply IHpi2; [ cbn; rewrite map_app | ]; reflexivity.
-      -- symmetry; apply Permutation_Type_middle.
+      -- symmetry. apply Permutation_Type_middle.
   + rewrite ? app_assoc.
     apply Permutation_Type_cons_app, Permutation_Type_app_tail, Permutation_Type_app_comm.
-- symmetry in Heql0; decomp_map_inf Heql0; subst.
+- symmetry in Heql0. decomp_map_inf Heql0. subst.
   destruct x; inversion Heql0.
-- symmetry in Heql0; decomp_map_inf Heql0; subst.
-  destruct x; inversion Heql0; subst.
+- symmetry in Heql0. decomp_map_inf Heql0. subst.
+  destruct x; inversion Heql0. subst.
   eapply ex_ir.
   + apply with_ilr1.
     eapply (@ex_ir _ (x1 :: l0 ++ l4)).
     * apply (IHpi (l0 ++ x1 :: l4)); [ cbn; rewrite map_app | ]; reflexivity.
-    * symmetry; apply Permutation_Type_middle.
+    * symmetry. apply Permutation_Type_middle.
   + apply Permutation_Type_middle.
-- symmetry in Heql0; decomp_map_inf Heql0; subst.
-  destruct x; inversion Heql0; subst.
+- symmetry in Heql0. decomp_map_inf Heql0. subst.
+  destruct x; inversion Heql0. subst.
   eapply ex_ir.
   + apply with_ilr2.
     eapply (@ex_ir _ (x2 :: l0 ++ l4)).
     * apply (IHpi (l0 ++ x2 :: l4)); [ cbn; rewrite map_app | ]; reflexivity.
-    * symmetry; apply Permutation_Type_middle.
+    * symmetry. apply Permutation_Type_middle.
   + apply Permutation_Type_middle.
-- symmetry in Heql0; decomp_map_inf Heql0; subst.
-  destruct x; inversion Heql0; subst.
+- symmetry in Heql0. decomp_map_inf Heql0. subst.
+  destruct x; inversion Heql0. subst.
   eapply ex_ir.
   + eapply (zero_ilr (l0 ++ l4)).
   + apply Permutation_Type_middle.
-- symmetry in Heql0; decomp_map_inf Heql0; subst.
-  destruct x; inversion Heql0; subst.
+- symmetry in Heql0. decomp_map_inf Heql0. subst.
+  destruct x; inversion Heql0. subst.
   eapply ex_ir.
   + apply plus_ilr.
     * eapply (@ex_ir _ (x1 :: l0 ++ l4)).
       -- apply (IHpi1 (l0 ++ x1 :: l4)); [ cbn; rewrite map_app | ]; reflexivity.
-      -- symmetry; apply Permutation_Type_middle.
+      -- symmetry. apply Permutation_Type_middle.
     * eapply (@ex_ir _ (x2 :: l0 ++ l4)).
       -- apply (IHpi2 (l0 ++ x2 :: l4)); [ cbn; rewrite map_app | ]; reflexivity.
-      -- symmetry; apply Permutation_Type_middle.
+      -- symmetry. apply Permutation_Type_middle.
   + apply Permutation_Type_middle.
-- destruct A'; inversion HeqA0; subst.
-  apply ill2ill_map_ioc_inv in Heql0.
-  destruct Heql0 as (l'' & -> & ->).
-  apply oc_irr.
-  apply IHpi; [ | reflexivity ].
-  symmetry; apply ill2ill_map_ioc.
-- symmetry in Heql0; decomp_map_inf Heql0; subst.
-  destruct x; inversion Heql0; subst.
+- destruct A'; inversion HeqA0. subst.
+  apply ill2ill_map_ioc_inv in Heql0 as [l'' -> -> ].
+  apply oc_irr, IHpi; [ | reflexivity ].
+  symmetry. apply ill2ill_map_ioc.
+- symmetry in Heql0. decomp_map_inf Heql0. subst.
+  destruct x; inversion Heql0. subst.
   eapply ex_ir.
   + apply de_ilr.
     eapply (@ex_ir _ (x :: l0 ++ l4)).
     * apply (IHpi (l0 ++ x :: l4)); [ cbn; rewrite map_app | ]; reflexivity.
-    * symmetry; apply Permutation_Type_middle.
+    * symmetry. apply Permutation_Type_middle.
   + apply Permutation_Type_middle.
-- symmetry in Heql0; decomp_map_inf Heql0; subst.
-  destruct x; inversion Heql0; subst.
+- symmetry in Heql0. decomp_map_inf Heql0. subst.
+  destruct x; inversion Heql0. subst.
   eapply ex_ir.
   + apply wk_ilr.
     apply (IHpi (l0 ++ l4)); [ cbn; rewrite map_app | ]; reflexivity.
   + apply Permutation_Type_middle.
-- symmetry in Heql0; decomp_map_inf Heql0; subst.
-  destruct x; inversion Heql0; subst.
+- symmetry in Heql0. decomp_map_inf Heql0. subst.
+  destruct x; inversion Heql0. subst.
   eapply ex_ir.
   + apply co_ilr.
     eapply (@ex_ir _ (ioc x :: ioc x :: l0 ++ l4)).
     * apply (IHpi (l0 ++ ioc x :: ioc x :: l4)); [ cbn; rewrite map_app | ]; reflexivity.
-    * symmetry; etransitivity;
-        [ apply Permutation_Type_cons_app, Permutation_Type_cons_app | ]; reflexivity.
+    * symmetry.
+      etransitivity; [ apply Permutation_Type_cons_app, Permutation_Type_cons_app | ]; reflexivity.
   + apply Permutation_Type_middle.
 - destruct a.
 Qed.
